src/tactic/hammer/mex2.lean
@@ -4,6 +4,6 @@ import tactic.hammer.monomorphization data.nat.gcd data.real.basic
 set_option trace.super true
 
 example (x y : ℝ) (h : x < y) : ∃ z : ℚ, x < z ∧ (z : ℝ) ≤ y :=
-by hammer_via_monom 60
+by hammer2 60
 -- by feature_search
--- by find_lemmas_via_monom [real.archimedean, exists_rat_btwn]
+-- by find_lemmas2 [real.archimedean, exists_rat_btwn]
