src/tactic/hammer/mex3.lean
@@ -5,4 +5,4 @@ set_option trace.super true
 
 example {α} [linear_ordered_field α] [archimedean α] {x y : α} (h : x < y) :
   ∃ q : ℚ, x < q ∧ (q:α) < y :=
-by hammer_via_monom
+by hammer2
