src/tactic/hammer/mex4.lean
@@ -4,4 +4,4 @@ import tactic.hammer.monomorphization data.nat.gcd data.real.basic
 set_option trace.super true
 
 example (x y : ℕ ) : x > y ∨ x ≤ y :=
-by hammer_via_monom
+by hammer2
