src/tactic/hammer/mex8.lean
@@ -3,7 +3,7 @@ import tactic.hammer.monomorphization data.nat.gcd data.real.basic
 -- set_option profiler true
 set_option trace.super true
 example (x y : ℕ) : x ∣ x * y :=
-by hammer_via_monom
+by hammer2
 -- by feature_search
--- by find_lemmas_via_monom [dvd_mul_right]
--- by find_lemmas_via_monom [dvd_mul_right, foo, foo'] -- [nat.gcd_dvd]
+-- by find_lemmas2 [dvd_mul_right]
+-- by find_lemmas2 [dvd_mul_right, foo, foo'] -- [nat.gcd_dvd]
